70

HumanEvalLean/HumanEval70.lean
@@ -1,7 +1,257 @@
 module
 
-def strange_sort_list : Unit :=
-  ()
+def strangeSortArray (xs : Array Int) : Array Int :=
+  let sorted := xs.toList.mergeSort.toArray
+  Array.ofFn (n := sorted.size)
+    (fun i => if i.val % 2 = 0 then sorted[i.val / 2] else sorted[sorted.size - 1 - i.val / 2])
+
+theorem t {xs : List Int} :
+    xs.min?.all (· ∈ xs) := by
+  simp only [Option.all_eq_true_iff_get]
+  grind
+
+grind_pattern t => xs.min?
+
+def strangeSortListSlow (xs : List Int) : List Int :=
+    match _ : xs.min? with
+    | some minimum =>
+      let xs' := xs.erase minimum
+      minimum :: (strangeSortListSlow xs'.reverse).reverse
+    | none => []
+termination_by xs.length
+decreasing_by grind
+
+theorem strangeSortArray_empty :
+    strangeSortArray #[] = #[] := by
+  grind [strangeSortArray, List.mergeSort_nil]
+
+theorem strangeSortArray_singleton :
+    strangeSortArray #[x] = #[x] := by
+  ext <;> grind [strangeSortArray, List.mergeSort_singleton, Array.size_ofFn, Array.getElem_ofFn]
+
+theorem List.Perm.min_eq [LE α] [Min α] [Std.LawfulOrderMin α] [Std.IsLinearOrder α]
+    {xs ys : List α} (h_perm : xs.Perm ys) (h : xs ≠ []) :
+    xs.min h = ys.min (by grind [Perm.eq_nil]) := by
+  simp only [List.min_eq_iff]
+  grind
+
+theorem List.Perm.min?_eq [LE α] [Min α] [Std.LawfulOrderMin α] [Std.IsLinearOrder α]
+    {xs ys : List α} (h_perm : xs.Perm ys) :
+    xs.min? = ys.min? := by
+  match xs, ys with
+  | [], [] => rfl
+  | x :: xs, y :: ys =>
+    rw [min?_eq_some_min, min?_eq_some_min, h_perm.min_eq]
+    simp
+  | x :: xs, [] | [], y :: ys => grind [Perm.nil_eq, Perm.eq_nil]
+
+theorem List.Perm.max_eq [LE α] [Max α] [Std.LawfulOrderMax α] [Std.IsLinearOrder α]
+    {xs ys : List α} (h_perm : xs.Perm ys) (h : xs ≠ []) :
+    xs.max h = ys.max (by grind [Perm.eq_nil]) := by
+  simp only [List.max_eq_iff]
+  grind
+
+theorem List.Perm.max?_eq [LE α] [Max α] [Std.LawfulOrderMax α] [Std.IsLinearOrder α]
+    {xs ys : List α} (h_perm : xs.Perm ys) :
+    xs.max? = ys.max? := by
+  match xs, ys with
+  | [], [] => rfl
+  | x :: xs, y :: ys =>
+    rw [max?_eq_some_max, max?_eq_some_max, h_perm.max_eq]
+    simp
+  | x :: xs, [] | [], y :: ys => grind [Perm.nil_eq, Perm.eq_nil]
+
+theorem List.foldl_concat [Max α] {xs : List α} :
+    (xs.concat x).foldl f init = f (xs.foldl f init) x := by
+  simp
+
+-- theorem List.max?_concat [Max α] {xs : List α} :
+--     (xs.concat x).max? = xs.max?.elim x (fun maximum => max maximum x) := by
+--   induction xs
+--   sorry
+
+-- theorem List.max?_eq_getLast? [Max α] {xs : List α} (hp : xs.Pairwise (fun a b => max a b = b)) :
+--     xs.max? = xs.getLast? := by
+--   rw [← List.reverse_reverse (as := xs)]
+--   generalize xs.reverse = xs
+--   induction xs
+--   · simp
+--   · rename_i x xs ih
+--     simp [List.max?_push, List.getLast?_cons]
+
+theorem List.max_eq_getLast [Max α] {xs : List α} (h) (hp : xs.Pairwise (fun a b => max a b = b)) :
+    xs.max h = xs.getLast h := by
+  rw [List.max.eq_def]
+  split
+  rename_i x xs _
+  suffices ∀ xs : List α, (x :: xs.reverse).Pairwise (fun a b => max a b = b) → foldl max x xs.reverse = (x :: xs.reverse).getLast (by grind) by
+    simp +singlePass only [← List.reverse_reverse (as := xs)]
+    grind
+  simp [- pairwise_cons]
+  intro xs hp
+  induction xs
+  · simp
+  · simp
+    rename_i ih
+    rw [ih]
+    rw [List.reverse_cons, ← List.cons_append, pairwise_append] at hp <;> grind
+    grind -- what's going on?
+
+theorem Array.max_eq_back [Max α] {xs : Array α} (h) (hp : xs.toList.Pairwise (fun a b => max a b = b)) :
+    xs.max h = xs.back (by grind) := by
+  rw [← max_toList, List.max_eq_getLast, getLast_toList]
+  · exact hp
+  · simp [h]
+
+theorem List.max?_eq_getLast? [Max α] {xs : List α} (hp : xs.Pairwise (fun a b => max a b = b)) :
+    xs.max? = xs.getLast? := by
+  cases xs
+  · simp
+  · rw [max?_eq_some_max, max_eq_getLast, getLast?_eq_some_getLast]
+    · simp
+    · exact hp
+
+theorem Std.min_eq_left_iff [LE α] [Min α] [Std.Refl (α := α) (· ≤ ·)]
+    [Std.LawfulOrderLeftLeaningMin α] {a b : α} :
+    min a b = a ↔ a ≤ b := by
+  by_cases a ≤ b
+  · grind [Std.LawfulOrderLeftLeaningMin.min_eq_left]
+  · rename_i h
+    simp only [Std.LawfulOrderLeftLeaningMin.min_eq_right _ _ h, iff_false, h]
+    rintro rfl
+    exact h.elim (Std.Refl.refl _)
+
+theorem Std.max_eq_right_iff [LE α] [Max α] [Std.IsLinearOrder α] [Std.LawfulOrderMax α]
+    {a b : α} :
+    max a b = b ↔ a ≤ b := by
+  open scoped Classical in grind [max_eq_if]
+
+theorem List.getElem_zero_mergeSort {xs : List Int} (h) :
+    xs.mergeSort[0]'h = xs.min (by grind [length_mergeSort]) := by
+  rw [(xs.mergeSort_perm (· ≤ ·)).symm.min_eq, List.min_eq_head, List.head_eq_getElem]
+  simp only [Std.min_eq_left_iff]
+  simpa using xs.pairwise_mergeSort (by grind) (by grind) (le := (· ≤ ·))
+
+theorem List.getElem_length_sub_one_mergeSort {xs : List Int} (h) :
+    xs.mergeSort[xs.length - 1]'h = xs.max (by grind [length_mergeSort]) := by
+  rw [(xs.mergeSort_perm (· ≤ ·)).symm.max_eq, List.max_eq_getLast, List.getLast_eq_getElem]
+  · simp [List.length_mergeSort]
+  · simp only [Std.max_eq_right_iff]
+    simpa using xs.pairwise_mergeSort (by grind) (by grind) (le := (· ≤ ·))
+
+theorem List.max_erase_le_max {xs : List Int} (h) :
+    (xs.erase x).max h ≤ xs.max (by grind) := by
+  simp only [List.max_le_iff]
+  intro b hb
+  apply List.le_max_of_mem
+  exact List.mem_of_mem_erase hb
+
+theorem Array.max_erase_le_max {xs : Array Int} {h} :
+    (xs.erase x).max h ≤ xs.max (by grind) := by
+  simp only [Array.max_le_iff]
+  intro b hb
+  apply Array.le_max_of_mem
+  exact Array.mem_of_mem_erase hb
+
+theorem List.count_dropLast [BEq α] {xs : List α} {a : α} :
+    xs.dropLast.count a = xs.count a - if xs.getLast? == some a then 1 else 0 := by
+  rw [← List.reverse_reverse (as := xs)]
+  generalize xs.reverse = xs
+  rw [dropLast_reverse, count_reverse, count_tail, getLast?_reverse, count_reverse]
+
+theorem Array.count_pop [BEq α] {xs : Array α} {a : α} :
+    xs.pop.count a = xs.count a - if xs.back? == some a then 1 else 0 := by
+  rw [← count_toList, toList_pop, List.count_dropLast, getLast?_toList, count_toList]
+
+theorem bla {xs : Array Int} {h} :
+    (xs.erase (xs.max h)).Perm xs.toList.mergeSort.toArray.pop := by
+  simp only [Array.perm_iff_toList_perm]
+  simp [List.perm_iff_count, Array.count_toList, - List.pop_toArray, - Array.toList_pop]
+  intro a
+  rw [Array.count_erase]
+  have h_mem : xs.max h ∈ xs := by grind
+  rw [Array.count_pop, List.count_toArray, List.count_toArray, (List.mergeSort_perm _ _).count_eq,
+    List.back?_toArray, ← List.max?_eq_getLast?, (List.mergeSort_perm _ _).max?_eq, Array.max?_toList,
+    Array.max?_eq_some_max]
+  · simp
+  · grind
+  · simp only [Std.max_eq_right_iff]
+    simpa using List.pairwise_mergeSort (α := Int) (le := (· ≤ ·)) (by grind) (by grind) _
+
+theorem bla' {xs : Array Int} {h} :
+    (xs.erase (xs.max h)).toList.mergeSort = xs.toList.mergeSort.dropLast := by
+  apply List.Perm.eq_of_pairwise (le := (· ≤ ·))
+  · grind
+  · simpa using List.pairwise_mergeSort (α := Int) (le := (· ≤ ·)) (by grind) (by grind) _
+  · simp only [List.dropLast_eq_take]
+    apply List.Pairwise.take
+    simpa using List.pairwise_mergeSort (α := Int) (le := (· ≤ ·)) (by grind) (by grind) _
+  · refine List.Perm.trans (List.mergeSort_perm _ _) ?_
+    rw [← Array.perm_iff_toList_perm]
+    apply bla
+
+theorem blub' {xs : Array Int} {h} :
+    (xs.erase (xs.min h)).toList.mergeSort = xs.toList.mergeSort.drop 1 := by
+  apply List.Perm.eq_of_pairwise (le := (· ≤ ·))
+  · grind
+  · simpa using List.pairwise_mergeSort (α := Int) (le := (· ≤ ·)) (by grind) (by grind) _
+  · apply List.Pairwise.drop
+    simpa using List.pairwise_mergeSort (α := Int) (le := (· ≤ ·)) (by grind) (by grind) _
+  · refine List.Perm.trans (List.mergeSort_perm _ _) ?_
+    rw [← Array.perm_iff_toList_perm]
+    simp only [Array.perm_iff_toList_perm]
+    simp [List.perm_iff_count, Array.count_toList, - List.pop_toArray, - Array.toList_pop]
+    intro a
+    rw [Array.count_erase]
+    have h_mem : xs.max h ∈ xs := by grind
+    rw [List.count_tail, List.count_toArray, (List.mergeSort_perm _ _).count_eq,
+      ← List.min?_eq_head?, (List.mergeSort_perm _ _).min?_eq, Array.min?_toList,
+      Array.min?_eq_some_min]
+    · simp
+    · grind
+    · simp only [Std.min_eq_left_iff]
+      simpa using List.pairwise_mergeSort (α := Int) (le := (· ≤ ·)) (by grind) (by grind) _
+
+theorem size_strangeSortArray {xs : Array Int} :
+    (strangeSortArray xs).size = xs.size := by
+  simp [strangeSortArray]
+
+theorem strangeSortArray_of_two_le_size (h : 2 ≤ xs.size) :
+    let minimum := xs.min (by grind)
+    let withoutMin := xs.erase minimum
+    let maximum := withoutMin.max (by grind)
+    let withoutMinMax := withoutMin.erase maximum
+    strangeSortArray xs = #[minimum, maximum] ++ strangeSortArray withoutMinMax := by
+  intro minimum withoutMin maximum withoutMinMax
+  ext
+  · simp [strangeSortArray]
+    grind
+  · rename_i i h₁ h₂
+    simp [strangeSortArray]
+    match i with
+    | 0 => grind [List.getElem_zero_mergeSort]
+    | 1 =>
+      simp [← Array.length_toList, List.getElem_length_sub_one_mergeSort, maximum, withoutMin]
+      rw [Array.max_eq_iff]
+      constructor
+      · grind [Array.mem_of_mem_erase]
+      · intro b hb
+        by_cases hb' : b = minimum
+        · cases hb'
+          simp only [minimum]
+          apply Array.min_le_of_mem
+          exact Array.mem_of_mem_erase (Array.max_mem _)
+        · apply Array.le_max_of_mem
+          rwa [Array.mem_erase_of_ne]
+          assumption
+    | j + 2 =>
+      have : withoutMinMax.toList.mergeSort = xs.toList.mergeSort.extract 1 (xs.toList.mergeSort.length - 1) := by
+        simp only [withoutMinMax, maximum, bla']
+        simp only [withoutMin, minimum, blub']
+        simp only [List.extract_eq_take_drop, List.dropLast_eq_take]
+        grind
+      simp [this]
+      grind [size_strangeSortArray]
 
 /-!
 ## Prompt
